Mostly finish dependently typed parser

src/Parsers/NonComputational.v
@@ -108,8 +108,13 @@ Section recursive_descent_parser.
       Context (H_prod_split : forall str0 str valid prod, H_prod_split_T str0 str valid prod (split_string_for_production str)).
 
       Context (lift_parse_name_success_lt : forall {str0 str : StringWithSplitState String split_stateT} {valid name}, Length str < Length str0 -> @T_productions_success str str initial_names_data (Lookup G name) -> @T_name_success str0 str valid name)
+              (lift_parse_name_failure_lt : forall {str0 str : StringWithSplitState String split_stateT} {valid name}, Length str < Length str0 -> @T_productions_failure str str initial_names_data (Lookup G name) -> @T_name_failure str0 str valid name)
               (lift_parse_name_success_eq : forall {str0 str : StringWithSplitState String split_stateT} {valid name},
-                                              str0 = str -> is_valid_name valid name = true -> @T_productions_success str0 str (remove_name valid name) (Lookup G name) -> @T_name_success str0 str valid name).
+                                              str = str0 :> String -> is_valid_name valid name = true -> @T_productions_success str0 str0 (remove_name valid name) (Lookup G name) -> @T_name_success str0 str valid name)
+              (lift_parse_name_failure_eq : forall {str0 str : StringWithSplitState String split_stateT} {valid name},
+                                              ~Length str < Length str0 -> @T_productions_failure str0 str0 (remove_name valid name) (Lookup G name) -> @T_name_failure str0 str valid name)
+              (elim_parse_name_failure : forall {str0 str : StringWithSplitState String split_stateT} {valid name},
+                                           str ≤s str0 -> ~ Length str < Length str0 -> is_valid_name valid name = false -> @T_name_failure str0 str valid name).
 
       Section item.
         Context (str0 str : StringWithSplitState String split_stateT)
@@ -264,14 +269,14 @@ Section recursive_descent_parser.
       End production_and_productions.
 
       Section names.
-        Context (str0 : StringWithSplitState String split_stateT)
-                (valid : names_listT).
-
-        Let T_productions := fun str prods => sum (T_productions_success str0 str valid prods) (T_productions_failure str0 str valid prods).
+        Let T_productions := fun str0 str valid prods => sum (T_productions_success str0 str valid prods) (T_productions_failure str0 str valid prods).
 
         Let T_name := fun str0 str valid name => sum (@T_name_success str0 str valid name) (@T_name_failure str0 str valid name).
 
         Section step.
+          Context (str0 : StringWithSplitState String split_stateT)
+                  (valid : names_listT).
+
           Context (parse_name
                    : forall (p : StringWithSplitState String split_stateT * names_listT),
                        prod_relation (ltof _ (fun s : StringWithSplitState _ _ => Length s)) names_listT_R p (str0, valid)
@@ -295,108 +300,104 @@ Section recursive_descent_parser.
                                 (or_intror eq_refl)
                                 (Lookup G name)) with
                          | inl success => inl (@lift_parse_name_success_lt str0 str valid name pf' success)
-                         | inr failure => inr _
+                         | inr failure => inr (@lift_parse_name_failure_lt str0 str valid name pf' failure)
                        end
                      | right pf', left H' =>
                        (** [str] didn't get smaller, so we cache the fact that we've hit this name already *)
                        (** It was valid, so we can remove it *)
-                       _ (*parse_productions
-                           _
-                           (@parse_name
-                              (str0, remove_name valid_list name)
-                              (or_intror (conj eq_refl (remove_name_dec H'))))
-                           _
-                           (or_intror eq_refl)
-                           (Lookup G name) *)
-                     | right _, right _
+                       match (parse_productions
+                                (@parse_name
+                                   (str0, remove_name valid name)
+                                   (or_intror (conj eq_refl (remove_name_dec H'))))
+                                _
+                                (or_intror eq_refl)
+                                (Lookup G name)) with
+                         | inl success => inl (@lift_parse_name_success_eq _ _ _ _ _ H' success)
+                         | inr failure => inr (@lift_parse_name_failure_eq _ _ _ _ pf' failure)
+                       end
+                     | right pf', right pf''
                        => (** oops, we already saw this name in the past.  ABORT! *)
-                       _ (*false*)
-                   end.
-            simpl in *.
+                         inr (@elim_parse_name_failure _ _ _ _ pf pf' pf'')
+                   end;
+            try solve [ destruct_head_hnf or; try assumption; exfalso; eauto with nocore ].
+          Defined.
+        End step.
 
-            hnf.
-
-            ).
-             End step.
-
-             Section wf.
-               (** TODO: add comment explaining signature *)
-               Definition parse_name_or_abort
-               : forall (p : StringWithSplitState String split_stateT * names_listT) (str : StringWithSplitState String split_stateT),
-                   str ≤s fst p
-                   -> string
-                   -> bool
-                 := @Fix3
-                      (prod (StringWithSplitState String split_stateT) names_listT) _ _ _
-                      _ (@well_founded_prod_relation
-                           (StringWithSplitState String split_stateT)
-                           names_listT
-                           _
-                           _
-                           (well_founded_ltof _ (fun s : StringWithSplitState String split_stateT => Length s))
-                           ntl_wf)
+        Section wf.
+          (** TODO: add comment explaining signature *)
+          Definition parse_name_or_abort
+          : forall (p : StringWithSplitState String split_stateT * names_listT) (str : StringWithSplitState String split_stateT)
+                   (pf : str ≤s fst p)
+                   (name : string),
+              T_name (fst p) str (snd p) name
+            := @Fix3
+                 (prod (StringWithSplitState String split_stateT) names_listT) _ _ _
+                 _ (@well_founded_prod_relation
+                      (StringWithSplitState String split_stateT)
+                      names_listT
                       _
-                      (fun sl => @parse_name_step (fst sl) (snd sl)).
+                      _
+                      (well_founded_ltof _ (fun s : StringWithSplitState String split_stateT => Length s))
+                      ntl_wf)
+                 _
+                 (fun sl => @parse_name_step (fst sl) (snd sl)).
 
-               Definition parse_name (str : StringWithSplitState String split_stateT) (name : string)
-               : bool
-                 := @parse_name_or_abort (str, initial_names_data) str
-                                         (or_intror eq_refl) name.
-             End wf.
-             End names.
-             End parts.
+          Definition parse_name (str : StringWithSplitState String split_stateT) (name : string)
+          : T_name str str initial_names_data name
+            := @parse_name_or_abort (str, initial_names_data) str
+                                    (or_intror eq_refl) name.
+        End wf.
+      End names.
+    End parts.
+  End generic.
 
-             End parts.
-             End generic.
+  Require Import Parsers.MinimalParse.
+  Section minimal.
+    Local Ltac t' :=
+      idtac;
+      match goal with
+        | _ => intro
+        | _ => progress hnf in *
+        | _ => progress simpl in *
+        | _ => progress subst_body
+        | _ => progress subst
+        | [ H : ?A -> ?B, H' : ?A |- _ ] => specialize (H H')
+        | [ H : ?A -> ?B |- _ ] => let A' := (eval hnf in A) in
+                                   progress change (A' -> B) in H
+        | _ => progress destruct_head StringWithSplitState
+        | _ => progress destruct_head False
+        | [ H : context[?x =s ?x] |- _ ]
+          => rewrite (proj2 (bool_eq_correct _ x x) eq_refl) in H
+        | [ H : true = false |- _ ] => exfalso; discriminate
+        | _ => progress inversion_head @minimal_parse_of_item
+        | _ => progress inversion_head @minimal_parse_of_production
+      end.
 
-             Require Import Parsers.MinimalParse.
-             Section minimal.
-               Local Ltac t' :=
-                 idtac;
-                 match goal with
-                   | _ => intro
-                   | _ => progress hnf in *
-                   | _ => progress simpl in *
-                   | _ => progress subst_body
-                   | _ => progress subst
-                   | [ H : ?A -> ?B, H' : ?A |- _ ] => specialize (H H')
-                   | [ H : ?A -> ?B |- _ ] => let A' := (eval hnf in A) in
-                                              progress change (A' -> B) in H
-                   | _ => progress destruct_head StringWithSplitState
-                   | _ => progress destruct_head False
-                   | [ H : context[?x =s ?x] |- _ ]
-                     => rewrite (proj2 (bool_eq_correct _ x x) eq_refl) in H
-                   | [ H : true = false |- _ ] => exfalso; discriminate
-                   | _ => progress inversion_head @minimal_parse_of_item
-                   | _ => progress inversion_head @minimal_parse_of_production
-                 end.
+    Local Ltac t := repeat t'.
 
-               Local Ltac t := repeat t'.
+    Section parts.
+      Section common.
+        Section with_str0_str_valid.
+          Context (str0 str : StringWithSplitState String split_stateT)
+                  (valid : names_listT).
 
-               Section parts.
-                 Section common.
-                   Context {str0 : StringWithSplitState String split_stateT}
-                           {valid : names_listT}.
-                   Section with_str.
-                     Context {str : StringWithSplitState String split_stateT}.
+          Definition T_name_success  (name : string) : Type
+            := minimal_parse_of_name String G initial_names_data is_valid_name remove_name
+                                     str0 valid str name.
+          Definition T_name_failure (name : string) : Type
+            := T_name_success name -> False.
 
-                     Definition T_name_success (name : string) : Type
-                       := minimal_parse_of_name String G initial_names_data is_valid_name remove_name
-                                                str0 valid str name.
-                     Definition T_name_failure (name : string) : Type
-                       := T_name_success name -> False.
+          Definition T_item_success (it : item CharType) : Type
+            := minimal_parse_of_item String G initial_names_data is_valid_name remove_name
+                                     str0 valid str it.
+          Definition T_item_failure (it : item CharType) : Type
+            := T_item_success it -> False.
 
-                     Definition T_item_success (it : item CharType) : Type
-                       := minimal_parse_of_item String G initial_names_data is_valid_name remove_name
-                                                str0 valid str it.
-                     Definition T_item_failure (it : item CharType) : Type
-                       := T_item_success it -> False.
+          Definition lift_success name (H : T_name_success name) : T_item_success (NonTerminal _ name)
+            := MinParseNonTerminal H.
 
-                     Definition lift_success name (H : T_name_success name) : T_item_success (NonTerminal _ name)
-                       := MinParseNonTerminal H.
-
-                     Definition lift_failure name (H : T_name_failure name) : T_item_failure (NonTerminal _ name).
-                     Proof.
+          Definition lift_failure name (H : T_name_failure name) : T_item_failure (NonTerminal _ name).
+          Proof.
             clear -H; abstract t.
           Defined.
 
@@ -469,11 +470,11 @@ Section recursive_descent_parser.
             inversion H'; subst;
             eauto.
           Qed.
-        End with_str.
+        End with_str0_str_valid.
 
-        Definition cons_success (s1 s2 str : StringWithSplitState String split_stateT) (pf : str ≤s str0) (H : s1 ++ s2 =s str) it its
-                   (p_it : @T_item_success s1 it) (p_its : @T_production_success s2 its)
-        : @T_production_success str (it :: its).
+        Definition cons_success (str0 s1 s2 str : StringWithSplitState String split_stateT) (valid : names_listT) (pf : str ≤s str0) (H : s1 ++ s2 =s str) it its
+                   (p_it : @T_item_success str0 s1 valid it) (p_its : @T_production_success str0 s2 valid its)
+        : @T_production_success str0 str valid (it :: its).
         Proof.
           hnf in *.
           apply bool_eq_correct in H.
@@ -483,6 +484,7 @@ Section recursive_descent_parser.
         Defined.
 
         Definition split_list_completeT
+                   (str0 : StringWithSplitState String split_stateT)
                    valid1 valid2
                    (str : StringWithSplitState String split_stateT) (pf : str ≤s str0)
                    (split_list : list (StringWithSplitState String split_stateT * StringWithSplitState String split_stateT))
@@ -499,7 +501,10 @@ Section recursive_descent_parser.
                                            * (minimal_parse_of_production _ G initial_names_data is_valid_name remove_name str0 valid2 (snd s1s2) its) }%type)
              end.
 
-        Lemma H_prod_split'_helper (it : item CharType) (its : list (item CharType))
+        Lemma H_prod_split'_helper
+              (str0 : StringWithSplitState String split_stateT)
+              (valid : names_listT)
+              (it : item CharType) (its : list (item CharType))
               (str strs : StringWithSplitState String split_stateT)
               (p_it : minimal_parse_of_item String G initial_names_data is_valid_name remove_name str0 valid str it)
               (p_its : minimal_parse_of_production String G initial_names_data is_valid_name remove_name str0 valid strs its)
@@ -514,9 +519,9 @@ Section recursive_descent_parser.
                         (fun s1s2 =>
                            let s1 := fst s1s2 in
                            let s2 := snd s1s2 in
-                           ((@T_item_failure s1 it * @T_production_failure s2 its)
-                            + (@T_item_success s1 it * @T_production_failure s2 its)
-                            + (@T_item_failure s1 it * @T_production_success s2 its))%type)
+                           ((@T_item_failure str0 s1 valid it * @T_production_failure str0 s2 valid its)
+                            + (@T_item_success str0 s1 valid it * @T_production_failure str0 s2 valid its)
+                            + (@T_item_failure str0 s1 valid it * @T_production_success str0 s2 valid its))%type)
                         ls))
         : False.
         Proof.
@@ -528,9 +533,12 @@ Section recursive_descent_parser.
           eauto.
         Qed.
 
-        Definition H_prod_split' str pf it its
-                   (split_list_complete : @split_list_completeT valid valid str pf (split_string_for_production str (it::its)) (it::its))
-        : @split_string_lift_T str0 (@T_item_success) (@T_item_failure) (@T_production_success) (@T_production_failure) str it its (split_string_for_production str).
+        Definition H_prod_split'
+                   (str0 str : StringWithSplitState String split_stateT)
+                   (valid : names_listT)
+                   pf it its
+                   (split_list_complete : @split_list_completeT str0 valid valid str pf (split_string_for_production str (it::its)) (it::its))
+        : @split_string_lift_T (@T_item_success) (@T_item_failure) (@T_production_success) (@T_production_failure) str0 str valid it its (split_string_for_production str).
         Proof.
           clear -split_list_complete.
           intros H pf' H'; hnf in H', split_list_complete.
@@ -554,11 +562,14 @@ Section recursive_descent_parser.
           eapply H_prod_split'_helper; eassumption.
         Qed.
 
-        Definition H_prod_split str prod
-                   (split_list_complete : forall pf, @split_list_completeT valid valid str pf (split_string_for_production str prod) prod)
+        Definition H_prod_split''
+                   (str0 str : StringWithSplitState String split_stateT)
+                   (valid : names_listT)
+                   prod
+                   (split_list_complete : forall pf, @split_list_completeT str0 valid valid str pf (split_string_for_production str prod) prod)
         : match prod return Type with
             | nil => unit
-            | it::its => @split_string_lift_T str0 (@T_item_success) (@T_item_failure) (@T_production_success) (@T_production_failure) str it its (split_string_for_production str)
+            | it::its => @split_string_lift_T (@T_item_success) (@T_item_failure) (@T_production_success) (@T_production_failure) str0 str valid it its (split_string_for_production str)
           end.
         Proof.
           unfold split_string_lift_T.
@@ -566,994 +577,104 @@ Section recursive_descent_parser.
           { constructor. }
           { intro pf. apply H_prod_split' with (pf := pf); try apply split_list_complete; assumption. }
         Defined.
+
+        Definition H_prod_split
+                   (split_list_complete : forall str0 str valid prod pf, @split_list_completeT str0 valid valid str pf (split_string_for_production str prod) prod)
+                   str0 str valid prod :=
+          H_prod_split'' str0 str valid prod (split_list_complete str0 str valid prod).
+
+        Definition lift_parse_name_success_lt
+                   (str0 str : StringWithSplitState String split_stateT) valid name
+        : Length str < Length str0
+          -> @T_productions_success str str initial_names_data (Lookup G name)
+          -> @T_name_success str0 str valid name
+          := @MinParseNonTerminalStrLt _ _ _ _ _ _ _ _ _ _ _.
+
+        Definition lift_parse_name_success_eq
+                   (str0 str : StringWithSplitState String split_stateT)
+                   valid name
+                   (H : str = str0 :> String)
+                   (H' : is_valid_name valid name = true)
+                   (p : @T_productions_success str0 str0 (remove_name valid name) (Lookup G name))
+        : @T_name_success str0 str valid name.
+        Proof.
+          hnf; case (eq_sym H).
+          exact (@MinParseNonTerminalStrEq _ String G _ initial_names_data is_valid_name remove_name str0 valid name H' p).
+        Defined.
+
+        Definition lift_parse_name_failure_lt
+                   (str0 str : StringWithSplitState String split_stateT)
+                   valid name
+                   (pf : Length str < Length str0)
+                   (p : @T_productions_failure str str initial_names_data (Lookup G name))
+        : @T_name_failure str0 str valid name.
+        Proof.
+          clear -pf p.
+          intro p'.
+          apply p; clear p.
+          inversion p'; subst; try assumption.
+          destruct str, str0; simpl in *; subst.
+          exfalso; omega.
+        Qed.
+
+        Definition lift_parse_name_failure_eq
+                   (str0 str : StringWithSplitState String split_stateT)
+                   valid name
+                   (pf : ~Length str < Length str0)
+                   (p : @T_productions_failure str0 str0 (remove_name valid name) (Lookup G name))
+        : @T_name_failure str0 str valid name.
+        Proof.
+          clear -pf p.
+          intro p'.
+          apply p; clear p.
+          inversion p'; subst.
+          { exfalso; eauto. }
+          { destruct str, str0; simpl in *; subst.
+            assumption. }
+        Qed.
+
+        Definition elim_parse_name_failure
+                   (str0 str : StringWithSplitState String split_stateT)
+                   valid name
+                   (pf : str ≤s str0)
+                   (pf' : ~ Length str < Length str0)
+                   (H : is_valid_name valid name = false)
+        : @T_name_failure str0 str valid name.
+        Proof.
+          clear -pf pf' H.
+          intro p.
+          inversion p; subst; eauto.
+          congruence.
+        Qed.
       End common.
 
-      Section item.
-        Context (str0 : StringWithSplitState String split_stateT)
-                (valid : names_listT).
-        Context (str : StringWithSplitState String split_stateT).
-
-        Context (str_matches_name : forall name, sum (@T_name_success str0 valid str name) (@T_name_failure str0 valid str name)).
-
-        Let T_name := fun name => sum (@T_name_success str0 valid str name) (@T_name_failure str0 valid str name).
-        Let T_item := fun it => sum (@T_item_success str0 valid str it) (@T_item_failure str0 valid str it).
-
-        Definition minimal_parse_item (it : item CharType) : T_item it
-          := @parse_item str T_name_success T_name_failure T_item_success T_item_failure lift_success lift_failure parse_terminal_success parse_terminal_failure str_matches_name it.
-      End item.
-
-      Section production.
-        Context (str0 : StringWithSplitState String split_stateT)
-                (valid : names_listT).
-        Context (parse_name : forall (str : StringWithSplitState String split_stateT),
-                                str ≤s str0
-                                -> forall name,
-                                     sum (@T_name_success str0 valid str name) (@T_name_failure str0 valid str name)).
-        Context (split_list_complete : forall str pf prod, @split_list_completeT str0 valid valid str pf (split_string_for_production str prod) prod).
-
-        Let T_production := fun str prod => sum (@T_production_success str0 valid str prod) (@T_production_failure str0 valid str prod).
-
-        (** To match a [production], we must match all of its items.
-            But we may do so on any particular split. *)
-        Definition minimal_parse_production
-                 (str : StringWithSplitState String split_stateT)
-                 (pf : str ≤s str0)
-                 (prod : production CharType)
-        : T_production str prod
-          := @parse_production
-               str0
-               (@T_name_success str0 valid) (@T_name_failure str0 valid)
-               (@T_item_success str0 valid) (@T_item_failure str0 valid)
-               (@lift_success str0 valid) (@lift_failure str0 valid)
-               (@parse_terminal_success str0 valid)
-               (@parse_terminal_failure str0 valid)
-               (@T_production_success str0 valid)
-               (@T_production_failure str0 valid)
-               parse_name
-               (@parse_empty_success str0 valid)
-               (@parse_empty_failure str0 valid)
-               (@cons_success str0 valid)
-               str pf
-               (fun str prod => @H_prod_split str0 valid str prod (fun pf => split_list_complete str pf prod))
-               prod.
-      End production.
-
-      Section production.
-        Context (str0 : StringWithSplitState String split_stateT)
-                (valid : names_listT).
-        Context (parse_name : forall (str : StringWithSplitState String split_stateT),
-                                str ≤s str0
-                                -> forall name,
-                                     sum (@T_name_success str0 valid str name) (@T_name_failure str0 valid str name)).
-        Context (split_list_complete : forall str pf prod, @split_list_completeT str0 valid valid str pf (split_string_for_production str prod) prod).
-
-        Let T_production := fun str prod => sum (@T_production_success str0 valid str prod) (@T_production_failure str0 valid str prod).
-
-        (** To match a [production], we must match all of its items.
-            But we may do so on any particular split. *)
-        Definition minimal_parse_production
-                 (str : StringWithSplitState String split_stateT)
-                 (pf : str ≤s str0)
-                 (prod : production CharType)
-        : T_production str prod
-          := @parse_production
-               str0
-               (@T_name_success str0 valid) (@T_name_failure str0 valid)
-               (@T_item_success str0 valid) (@T_item_failure str0 valid)
-               (@lift_success str0 valid) (@lift_failure str0 valid)
-               (@parse_terminal_success str0 valid)
-               (@parse_terminal_failure str0 valid)
-               (@T_production_success str0 valid)
-               (@T_production_failure str0 valid)
-               parse_name
-               (@parse_empty_success str0 valid)
-               (@parse_empty_failure str0 valid)
-               (@cons_success str0 valid)
-               str pf
-               (fun str prod => @H_prod_split str0 valid str prod (fun pf => split_list_complete str pf prod))
-               prod.
-      End production.
-
+      Definition minimal_parse_name
+                 (split_list_complete
+                  : forall str0 str valid prod pf,
+                      @split_list_completeT str0 valid valid str pf (split_string_for_production str prod) prod)
+      : forall (str : StringWithSplitState String split_stateT)
+               (name : string),
+          sum (T_name_success str str initial_names_data name)
+              (T_name_failure str str initial_names_data name)
+        := @parse_name
+             T_name_success T_name_failure
+             T_item_success T_item_failure
+             lift_success lift_failure
+             parse_terminal_success
+             parse_terminal_failure
+             T_production_success
+             T_production_failure
+             parse_empty_success
+             parse_empty_failure
+             cons_success
+             T_productions_success T_productions_failure
+             fail_parse_nil_productions
+             lift_prods_success_head lift_prods_success_tail
+             lift_prods_failure
+             (H_prod_split split_list_complete)
+             lift_parse_name_success_lt lift_parse_name_failure_lt
+             lift_parse_name_success_eq lift_parse_name_failure_eq
+             elim_parse_name_failure.
     End parts.
   End minimal.
-
-
-
-
-
-
-
-
-    Context (T_success T_failure : String -> productions CharType -> Type)
-            (T_success_reverse_lookup : forall str name, T_success str (Lookup G name) -> T_success str [ [ NonTerminal _ name ] ])
-            (T_failure_reverse_lookup : forall str name, T_failure str (Lookup G name) -> T_failure str [ [ NonTerminal _ name ] ])
-            (transport_T_success_str : forall (s1 s2 : String) nt, s1 = s2 -> T_success s1 nt -> T_success s2 nt)
-            (transport_T_failure_str : forall (s1 s2 : String) nt, s1 = s2 -> T_failure s1 nt -> T_failure s2 nt).
-    Let T str nt := (T_success str nt + T_failure str nt)%type.
-    Let transport_T_str (s1 s2 : String) nt (H : s1 = s2) (p : T s1 nt) : T s2 nt :=
-      match p with
-        | inl p' => inl (transport_T_success_str H p')
-        | inr p' => inr (transport_T_failure_str H p')
-      end.
-    Let T_reverse_lookup str name (p : T str (Lookup G name)) : T str [ [ NonTerminal _ name ] ]
-      :=  match p with
-            | inl p' => inl (T_success_reverse_lookup _ p')
-            | inr p' => inr (T_failure_reverse_lookup _ p')
-          end.
-    Context (parse_production_by_picking
-             : forall str0
-                      (parse_production_from_split_list'
-                       : forall (strs : list { str : String | str ≤s str0 })
-                                (pat : production CharType),
-                           ilist (fun sp => T (proj1_sig (fst sp)) [ [ snd sp ] ]) (combine strs pat))
-                      (str : String)
-                      (pf : str ≤s str0)
-                      (pat : production CharType),
-                 T str [ pat ]).
-    Context (decide_leaf : forall str ch, T str [ [ Terminal ch ] ]).
-    Context (fold_productions : forall str (pats : productions CharType),
-                               ilist (fun pat => T str [ pat ]) pats
-                               -> T str pats).
-    Context (make_abort : forall str nt valid_list, @is_valid_productions str valid_list nt = false -> T_failure str nt).
-
-
-
-
-
-
-    Section parts.
-      Section item.
-        Context (str : String)
-                (parse_productions : forall nt, T str nt).
-
-        Definition parse_item it : T str [ [ it ] ]
-          := match it with
-               | Terminal ch => decide_leaf str ch
-               | NonTerminal name => T_reverse_lookup _ (parse_productions (Lookup G name))
-             end.
-      End item.
-
-      Section production.
-        Variable str0 : String.
-        Variable parse_productions : forall (str : String)
-                                            (pf : str ≤s str0)
-                                            nt, T str nt.
-
-        Definition parse_production_from_split_list
-                   (strs : list { str : String | str ≤s str0 })
-                   (pat : production CharType)
-        : ilist (fun sp => T (proj1_sig (fst sp)) [ [ snd sp ] ]) (combine strs pat)
-          := imap_list (fun sp => T (proj1_sig (fst sp)) [ [ snd sp ] ])
-                       (fun sp => parse_item (@parse_productions _ (proj2_sig (fst sp))) (snd sp))
-                       (combine strs pat).
-
-        Definition parse_production (str : String) (pf : str ≤s str0) (pat : production CharType)
-        : T str [ pat ]
-          := parse_production_by_picking parse_production_from_split_list pf pat.
-      End production.
-
-      Section productions.
-        Section step.
-          Variable str0 : String.
-          Variable parse_productions : forall (str : String)
-                                              (pf : str ≤s str0)
-                                              nt, T str nt.
-
-          Definition parse_productions_step (str : String) (pf : str ≤s str0) (nt : productions CharType)
-          : T str nt
-            := fold_productions (imap_list (fun pat => T str [ pat ])
-                                        (parse_production parse_productions pf)
-                                        nt).
-        End step.
-
-        Section wf.
-          Definition parse_productions_or_abort str0 str valid (valid_list : forall str, productions_listT str)
-                     (pf : str ≤s str0)
-                     (nt : productions CharType)
-          : T str nt.
-          Proof.
-            revert str pf nt.
-            change str0 with (projT1 (existT productions_listT str0 (valid_list str0))).
-            generalize (existT productions_listT str0 (valid_list str0)); clear str0 valid_list.
-            refine (@Fix (sigT productions_listT) _ (@well_founded_sigT_relation
-                                                       String
-                                                       productions_listT
-                                                       _
-                                                       _
-                                                       (well_founded_ltof _ Length)
-                                                       ntl_wf)
-                         _ _).
-            intros [str0 valid_list] parse_productions str pf nt; simpl in *.
-            destruct (lt_dec (Length str) (Length str0)) as [pf'|pf'];
-              [ | unfold str_le in *; assert (H : str0 = str) by intuition; apply (transport_T_str H); clear H ].
-            { (** [str] got smaller, so we reset the valid productions list *)
-              specialize (parse_productions
-                            (existT _ str (initial_productions_data str))
-                            (or_introl pf')); simpl in *.
-              exact (parse_productions_step parse_productions (or_intror eq_refl) nt). }
-            { (** [str] didn't get smaller, so we cache the fact that we've hit this productions already *)
-              case_eq (is_valid_productions valid_list nt).
-              { (** It was valid, so we can remove it *)
-                intro H'.
-                specialize (fun pf' => parse_productions
-                              (existT _ str0 (remove_productions valid_list nt))
-                              (or_intror (ex_intro _ eq_refl pf'))); simpl in *.
-                specialize (parse_productions (remove_productions_dec H')).
-                exact (parse_productions_step parse_productions (or_intror eq_refl) nt). }
-              { (** oops, we already saw this productions in the past.  ABORT! *)
-                intro; right; eapply make_abort; eassumption. } }
-          Defined.
-
-          Definition parse_productions str nt : T str nt
-            := @parse_productions_or_abort str str initial_productions_data
-                                           (or_intror eq_refl) nt.
-        End wf.
-      End productions.
-    End parts.
-  End generic.
-
-  Section parse_tree.
-    Local Hint Constructors parse_of parse_of_production parse_of_item : parse_tree.
-    Local Hint Resolve ParseHead ParseProductionSingleton : parse_tree.
-    Local Hint Extern 1 => apply ParseHead : parse_tree.
-    Local Hint Extern 0 (option (parse_of _ _ _ [])) => exact None : parse_tree.
-    Context (pick_productions
-             : forall (str : String)
-                      (pat : production CharType)
-                      (patH : Datatypes.length pat > 0),
-                 { ls : list { split : list { str_part : String | str_part ≤s str }
-                             | List.length split = List.length pat
-                               /\ fold_right Concat (Empty _) (map (@proj1_sig _ _) split) = str }
-                 | List.length ls <> 0 }).
-
-    Let aggregate str pats : list (parse_of String G str pats +
-                                   option (parse_of String G str pats -> False))
-                             -> parse_of String G str pats +
-                                option (parse_of String G str pats -> False).
-    Proof.
-      intro ls.
-      induction ls as [|x xs IHxs].
-      { right; exact None. }
-      { destruct x as [| [ ] ]; try solve [ left; assumption
-                                          | right; apply Some; assumption ].
-        apply IHxs. }
-    Defined.
-
-    Definition parse_tree_for : forall str nt, parse_of String G str nt + option (parse_of String G str nt -> False).
-    Proof with auto with parse_tree nocore.
-      apply (@parse_productions (fun str nt => parse_of _ G str nt)
-                                (fun str nt => option (parse_of _ G str nt -> False)))...
-      { intros str name [np|]; [ apply Some | exact None ].
-        revert np; clear; intros.
-        abstract (repeat match goal with
-                           | [ H : context[_ ++ Empty String] |- _ ] => rewrite RightId in H
-                           | [ H : ?T, H' : ?T -> False |- _ ] => destruct (H' H)
-                           | [ p : parse_of _ _ _ _ |- _ ] => (inversion p; subst; clear p)
-                           | [ p : parse_of_production _ _ _ _ |- _ ] => (inversion p; subst; clear p)
-                           | [ p : parse_of_item _ _ _ _ |- _ ] => (inversion p; subst; clear p)
-                         end). }
-        { intros; subst; assumption. }
-        { intros; subst; assumption. }
-        { intros str0 parse_production_from_split_list' str pf pat.
-          pose proof (parse_production_from_split_list' ((exist _ str pf)::nil) pat) as parse_production_from_split_list''; simpl in *.
-          destruct pat as [|pat0 [|pat1 pats] ]; simpl in *.
-          { case_eq (str =s Empty _); intro H; [ left | right; exact None ]...
-            apply bool_eq_correct in H; subst... }
-          { destruct (ilist_hd parse_production_from_split_list'') as [tree|]; simpl in *; [ left | right ]; assumption. }
-          { (** we need to split the string *)
-            clear parse_production_from_split_list''.
-            refine (aggregate _); clear aggregate.
-            refine (map _ (proj1_sig (@pick_productions str (pat0::pat1::pats) (Gt.gt_Sn_O _)))); clear pick_productions.
-            intros [ split [ split_length split_strings ] ].
-            let T := match type of split with list ?T => constr:(T) end in
-            set (f := (map (fun x' : T
-                      => exist
-                           (fun str => str ≤s str0)
-                           (proj1_sig x')
-                           (match pf, proj2_sig x' with
-                              | or_introl H0, or_introl H1 => or_introl (transitivity H1 H0)
-                              | or_introl H0, or_intror H1 => or_introl (transitivity (R := le) (Le.le_n_S _ _ (NPeano.Nat.eq_le_incl _ _ (f_equal Length H1))) H0)
-                              | or_intror H0, or_introl H1 => or_introl (transitivity (R := le) H1 (NPeano.Nat.eq_le_incl _ _ (f_equal Length H0)))
-                              | or_intror H0, or_intror H1 => or_intror (transitivity H1 H0)
-                            end)))).
-            specialize (parse_production_from_split_list' (f split) (pat0 :: pat1 :: pats)).
-            generalize dependent split.
-            intro split.
-            generalize (pat0::pat1::pats).
-            clear pat0 pat1 pats.
-            assert (H0 : Datatypes.length (f split) = Datatypes.length split)
-              by (clear; abstract (induction split; simpl; auto)).
-            assert (H1 : map (@proj1_sig _ _) (f split) = map (@proj1_sig _ _) split)
-              by (clear; abstract (induction split; simpl; f_equal; auto)).
-            rewrite <- H0; clear H0.
-            rewrite <- H1; clear H1.
-            generalize (f split); clear split; clear f.
-            intros fsplit pats.
-            clear pf.
-            revert pats str.
-            induction fsplit;
-              intro pats; intros;
-              destruct pats;
-              repeat match goal with
-                       | [ H : @eq nat _ _ |- _ ] => progress simpl in H
-                       | [ H : @eq nat _ _ |- _ ] => exfalso; revert H; clear; intro H; abstract inversion H
-                       | _ => progress subst
-                       | [ H : S _ = S _ |- _ ] => apply (f_equal pred) in H
-                       | [ H : ?x = ?x |- _ ] => clear H
-                     end.
-            { simpl in *; left; subst... }
-            { simpl in *.
-              let IHfsplit := match goal with
-                                | [ IHfsplit : forall pats str,
-                                                 ilist _ _ ->
-                                                 _ = _ ->
-                                                 fold_right _ _ _ = str ->
-                                                 _ + _
-                                                 |- _ ] => constr:IHfsplit
-                              end in
-              match goal with
-                | [ H : Datatypes.length _ = Datatypes.length _ |- _ ]
-                  => specialize (fun l => IHfsplit _ _ l H eq_refl)
-              end;
-                let ls := match goal with | [ ls : ilist _ (_::_) |- _ ] => constr:ls end in
-                specialize (IHfsplit (ilist_tl ls));
-                  let ls_hd := fresh "ls_hd" in
-                  pose proof (ilist_hd ls) as ls_hd;
-                    simpl in ls_hd;
-                    clear ls;
-                    refine (match ls_hd, IHfsplit with
-                              | inl p1, inl p2 => inl (ParseApp p1 p2)
-                              | inr _, _ => inr None
-                              | _, inr _ => inr None
-                            end). } } }
-      { (** decide_leaf *)
-        intros str ch.
-        case_eq (str =s [[ch]]); intro H; [ apply bool_eq_correct in H; left | right; exact None ].
-        subst... }
-      { (** fold_productions *)
-        intros str pats parses; induction parses; simpl in *;
-        repeat match goal with
-                 | [ H : option _ |- _ ] => destruct H
-                 | [ H : sum _ _ |- _ ] => destruct H
-               end;
-          try solve [ left; auto with parse_tree nocore
-                    | left;
-                      repeat match goal with
-                               | _ => progress auto with parse_tree nocore
-                               | [ H : parse_of _ _ _ _ |- _ ] => inversion H; clear H; subst
-                             end
-                    | match goal with
-                        | [ H : parse_of _ _ _ _ |- _ ] => fail 1
-                        | _ => idtac
-                      end;
-                      right; exact None
-                    | right;
-                      apply Some;
-                      let p := fresh in
-                      intro p; inversion p; clear p; subst;
-                      auto with parse_tree nocore ]. }
-      { (** make_abort *)
-        intros; exact None. }
-    Defined.
-  End parse_tree.
-
-
-(*  Section parse_tree_no_split.
-    Local Hint Constructors parse_of parse_of_production parse_of_item : parse_tree.
-    Local Hint Resolve ParseHead ParseProductionSingleton : parse_tree.
-    Local Hint Extern 1 => apply ParseHead : parse_tree.
-    Local Hint Extern 0 (option (parse_of _ _ _ [])) => exact None : parse_tree.
-
-    Definition parse_tree_no_split_for : forall str nt, option (parse_of String G str nt).
-    Proof with auto with parse_tree nocore.
-      apply (@parse_productions (fun str nt => option (parse_of _ G str nt))).
-      { intros str name [p|]; [ apply Some | exact None ]... }
-      { intros.
-        specialize (parse_production_from_split_list' ((exist _ str pf)::nil) pat); simpl in *.
-        destruct pat as [|pat0 [|pat1 pats] ]; simpl in *.
-        { case_eq (str =s Empty _); intro H; [ apply Some | exact None ]...
-          apply bool_eq_correct in H; subst... }
-        { destruct (ilist_hd parse_production_from_split_list') as [tree|]; simpl in *; [ apply Some | exact None ]... }
-        { (** we don't handle the case where we need to split the string *)
-          exact None. } }
-      { (** decide_leaf *)
-        intros str ch.
-        case_eq (str =s [[ch]]); intro H; [ apply bool_eq_correct in H; apply Some | exact None ].
-        subst... }
-      { (** fold_productions *)
-        intros str pats parses; induction parses; simpl in *...
-        repeat match goal with H : option _ |- _ => destruct H end;
-          try solve [ apply Some; auto with parse_tree nocore
-                    | apply Some;
-                      repeat match goal with
-                               | _ => progress auto with parse_tree nocore
-                               | [ H : parse_of _ _ _ _ |- _ ] => inversion H; clear H; subst
-                             end
-                    | match goal with
-                        | [ H : parse_of _ _ _ _ |- _ ] => fail 1
-                        | _ => idtac
-                      end;
-                      exact None ]. }
-      { (** make_abort *)
-        intros; exact None. }
-    Defined.
-  End parse_tree_no_split.
-
-
-
-
-  Section generic_by_simple_listing.
-    (** If we don't need to pass proofs down the tree, we can just ask for a list of splits. *)
-    Context (T_success T_failure : String -> productions CharType -> Type)
-            (T_success_reverse_lookup : forall str name, T_success str (Lookup G name) -> T_success str [ [ NonTerminal _ name ] ])
-            (T_failure_reverse_lookup : forall str name, T_failure str (Lookup G name) -> T_failure str [ [ NonTerminal _ name ] ])
-            (transport_T_success_str : forall (s1 s2 : String) nt, s1 = s2 -> T_success s1 nt -> T_success s2 nt)
-            (transport_T_failure_str : forall (s1 s2 : String) nt, s1 = s2 -> T_failure s1 nt -> T_failure s2 nt).
-    Let T str nt := (T_success str nt + T_failure str nt)%type.
-    Let transport_T_str (s1 s2 : String) nt (H : s1 = s2) (p : T s1 nt) : T s2 nt :=
-      match p with
-        | inl p' => inl (transport_T_success_str H p')
-        | inr p' => inr (transport_T_failure_str H p')
-      end.
-    Context (pick_productions
-             : forall (str : String)
-                      (pat : production CharType),
-                 { ls : list { split : list { str_part : String | Length _ str_part < Length _ str \/ str_part = str }
-                             | List.length split = List.length pat
-                               /\ fold_right (Concat _) (Empty _) (map (@proj1_sig _ _) split) = str }
-                 | List.length ls <> 0 }).
-    Context (simple_fold_production_parts
-             : forall str0
-                      strs
-                      (pat : production CharType)
-                      (pf : List.length strs = List.length pat),
-                 ilist (fun sp : {str1 : String |
-                                  Length String str1 < Length String str0 \/
-                                  str1 = str0} * item CharType
-                        => T (proj1_sig (fst sp)) [ [ snd sp ] ])
-                       (combine strs pat)
-                 -> T (fold_left (Concat _) (map (@proj1_sig _ _) strs) (Empty _))
-                      [ pat ]).
-    Context (decide_leaf : forall str ch, T str [ [ Terminal ch ] ]).
-    Context (fold_productions : forall str (pats : productions CharType),
-                               ilist (fun pat => T str [ pat ]) pats
-                               -> T str pats).
-    Context (make_abort : forall str nt valid_list, @is_valid_productions str valid_list nt = false -> T_failure str nt).
-
-    Definition parse_productions_with_split_picker str nt : T str nt.
-    Proof.
-      refine (@parse_productions T_success T_failure T_success_reverse_lookup T_failure_reverse_lookup transport_T_success_str transport_T_failure_str _ decide_leaf fold_productions make_abort str nt).
-      clear str nt.
-      intros str0 parse_a_split str H pat.
-      specialize (pick_productions str pat).
-      specialize (fun strs => parse_a_split strs pat).
-      specialize (fun strs H =>
-                    @simple_fold_production_parts _ _ _ H (parse_a_split strs)).
-      clear parse_a_split.
-      move simple_fold_production_parts at bottom.
-      specialize (fun strs pf1 pf2 =>
-                    @transport_T_str
-                      _ str _ pf1
-                      (@simple_fold_production_parts strs pf2)).
-      clear simple_fold_production_parts.
-      move pick_productions at bottom.
-      move transport_T_str at bottom.
-      destruct pick_productions as [ls H'].
-      let T := match type of ls with list (@sig (list ?T) _) => constr:(T) end in
-      set (f := (map (fun x' : T
-                      => exist
-                           (fun str => Length String str < Length String str0 \/ str = str0)
-                           (proj1_sig x')
-                           (match H, proj2_sig x' with
-                              | or_introl H0, or_introl H1 => or_introl (transitivity H1 H0)
-                              | or_introl H0, or_intror H1 => or_introl (transitivity (R := le) (Le.le_n_S _ _ (NPeano.Nat.eq_le_incl _ _ (f_equal (Length String) H1))) H0)
-                              | or_intror H0, or_introl H1 => or_introl (transitivity (R := le) H1 (NPeano.Nat.eq_le_incl _ _ (f_equal (Length String) H0)))
-                              | or_intror H0, or_intror H1 => or_intror (transitivity H1 H0)
-                            end)))).
-      pose proof (map f (map (@proj1_sig _ _) ls)).
-      let T := match type of ls with list ?T => constr:(T) end in
-      pose proof (@map
-                    T _
-                    f
-                    ls).
-
-      assert (forall B : Type, ({split
-       : list
-           {str_part : String |
-           Length String str_part < Length String str \/ str_part = str} |
-       Datatypes.length split = Datatypes.length pat /\
-       fold_left (Concat String)
-         (map
-            (proj1_sig
-               (P:=fun str_part : String =>
-                   Length String str_part < Length String str \/
-                   str_part = str)) split) (Empty String) = str} -> B)).
-      intros B x.
-      assert (list
-    {str_part : String |
-     Length String str_part < Length String str \/ str_part = str} ->
-              list {str : String | Length String str < Length String str0 \/ str = str0}).
-      refine .
-      SearchAbout (_ <= _ -> S _ <= S _).
-
-      refine (fun x' => _).
-      refine (map _
-                   pose proof (@transport_T_str (map (fun x' => exist _ (proj1_sig x') (proj1_sig x)).
- in parse
-
-
-
-      apply simple_fold_production_parts.
-
-      move pick_productions at bottom.
-      pose @imap_list.
-            := @parse_productions_or_abort str str initial_productions_data
-                                           (or_intror eq_refl) nt.
-
-  Section parse_tree_no_split.
-    Local Hint Constructors parse_of parse_of_production parse_of_item : parse_tree.
-    Local Hint Resolve ParseHead ParseProductionSingleton : parse_tree.
-    Local Hint Extern 1 => apply ParseHead : parse_tree.
-    Local Hint Extern 0 (option (parse_of _ _ _ [])) => exact None : parse_tree.
-
-    Definition parse_tree_no_split_for : forall str nt, option (parse_of String G str nt).
-    Proof with auto with parse_tree nocore.
-      apply (@parse_productions (fun str nt => option (parse_of _ G str nt))).
-      { intros str name [p|]; [ apply Some | exact None ]... }
-      { intros.
-        specialize (parse_production_from_split_list' ((exist _ str pf)::nil) pat); simpl in *.
-        destruct pat as [|pat0 [|pat1 pats] ]; simpl in *.
-        { case_eq (str =s Empty _); intro H; [ apply Some | exact None ]...
-          apply bool_eq_correct in H; subst... }
-        { destruct (ilist_hd parse_production_from_split_list') as [tree|]; simpl in *; [ apply Some | exact None ]... }
-        { (** we don't handle the case where we need to split the string *)
-          exact None. } }
-      { (** decide_leaf *)
-        intros str ch.
-        case_eq (str =s [[ch]]); intro H; [ apply bool_eq_correct in H; apply Some | exact None ].
-        subst... }
-      { (** fold_productions *)
-        intros str pats parses; induction parses; simpl in *...
-        repeat match goal with H : option _ |- _ => destruct H end;
-          try solve [ apply Some; auto with parse_tree nocore
-                    | apply Some;
-                      repeat match goal with
-                               | _ => progress auto with parse_tree nocore
-                               | [ H : parse_of _ _ _ _ |- _ ] => inversion H; clear H; subst
-                             end
-                    | match goal with
-                        | [ H : parse_of _ _ _ _ |- _ ] => fail 1
-                        | _ => idtac
-                      end;
-                      exact None ]. }
-      { (** make_abort *)
-        intros; exact None. }
-    Defined.
-  End parse_tree_no_split.
-
-
-  Section parse_tree_no_split.
-    Local Hint Constructors parse_of parse_of_production parse_of_item : parse_tree.
-    Local Hint Resolve ParseHead ParseProductionSingleton : parse_tree.
-    Local Hint Extern 1 => apply ParseHead : parse_tree.
-    Local Hint Extern 0 (option (parse_of _ _ _ [])) => exact None : parse_tree.
-
-    Definition parse_tree_no_split_for : forall str nt, option (parse_of String G str nt).
-    Proof with auto with parse_tree nocore.
-      apply (@parse_productions (fun str nt => option (parse_of _ G str nt))).
-      { intros str name [p|]; [ apply Some | exact None ]... }
-      { intros.
-        specialize (parse_production_from_split_list' ((exist _ str pf)::nil) pat); simpl in *.
-        destruct pat as [|pat0 [|pat1 pats] ]; simpl in *.
-        { case_eq (str =s Empty _); intro H; [ apply Some | exact None ]...
-          apply bool_eq_correct in H; subst... }
-        { destruct (ilist_hd parse_production_from_split_list') as [tree|]; simpl in *; [ apply Some | exact None ]... }
-        { (** we don't handle the case where we need to split the string *)
-          exact None. } }
-      { (** decide_leaf *)
-        intros str ch.
-        case_eq (str =s [[ch]]); intro H; [ apply bool_eq_correct in H; apply Some | exact None ].
-        subst... }
-      { (** fold_productions *)
-        intros str pats parses; induction parses; simpl in *...
-        repeat match goal with H : option _ |- _ => destruct H end;
-          try solve [ apply Some; auto with parse_tree nocore
-                    | apply Some;
-                      repeat match goal with
-                               | _ => progress auto with parse_tree nocore
-                               | [ H : parse_of _ _ _ _ |- _ ] => inversion H; clear H; subst
-                             end
-                    | match goal with
-                        | [ H : parse_of _ _ _ _ |- _ ] => fail 1
-                        | _ => idtac
-                      end;
-                      exact None ]. }
-      { (** make_abort *)
-        intros; exact None. }
-    Defined.
-  End parse_tree_no_split.*)
 End recursive_descent_parser.
-
-Section recursive_descent_parser_list.
-  Context {CharType} {String : string_like CharType} {G : grammar CharType}.
-  Variable (CharType_eq_dec : forall x y : CharType, {x = y} + {x <> y}).
-  Definition rdp_list_productions_listT : String -> Type := fun _ => list (productions CharType).
-  Definition rdp_list_is_valid_productions : forall str, rdp_list_productions_listT str -> productions CharType -> bool
-    := fun str ls nt => if in_dec (productions_dec CharType_eq_dec) nt ls then true else false.
-  Definition rdp_list_remove_productions : forall str, rdp_list_productions_listT str -> productions CharType -> rdp_list_productions_listT str
-    := fun str ls nt =>
-         filter (fun x => if productions_dec CharType_eq_dec nt x then false else true) ls.
-  Definition rdp_list_productions_listT_R : forall str, rdp_list_productions_listT str -> rdp_list_productions_listT str -> Prop
-    := fun _ => ltof _ (@List.length _).
-  Lemma filter_list_dec {T} f (ls : list T) : List.length (filter f ls) <= List.length ls.
-  Proof.
-    induction ls; trivial; simpl in *.
-    repeat match goal with
-             | [ |- context[if ?a then _ else _] ] => destruct a; simpl in *
-             | [ |- S _ <= S _ ] => solve [ apply Le.le_n_S; auto ]
-             | [ |- _ <= S _ ] => solve [ apply le_S; auto ]
-           end.
-  Defined.
-  Lemma rdp_list_remove_productions_dec : forall str ls nt, @rdp_list_is_valid_productions str ls nt = true
-                                                            -> @rdp_list_productions_listT_R str (@rdp_list_remove_productions str ls nt) ls.
-  Proof.
-    intros.
-    unfold rdp_list_is_valid_productions, rdp_list_productions_listT_R, rdp_list_remove_productions, ltof in *.
-    destruct (in_dec (productions_dec CharType_eq_dec) nt ls); [ | discriminate ].
-    match goal with
-      | [ H : In ?nt ?ls |- context[filter ?f ?ls] ]
-        => assert (~In nt (filter f ls))
-    end.
-    { intro H'.
-      apply filter_In in H'.
-      destruct H' as [? H'].
-      destruct (productions_dec CharType_eq_dec nt nt); congruence. }
-    { match goal with
-        | [ |- context[filter ?f ?ls] ] => generalize dependent f; intros
-      end.
-      induction ls; simpl in *; try congruence.
-      repeat match goal with
-               | [ |- context[if ?x then _ else _] ] => destruct x; simpl in *
-               | [ H : _ \/ _ |- _ ] => destruct H
-               | _ => progress subst
-               | [ H : ~(_ \/ _) |- _ ] => apply Decidable.not_or in H
-               | [ H : _ /\ _ |- _ ] => destruct H
-               | [ H : ?x <> ?x |- _ ] => exfalso; apply (H eq_refl)
-               | _ => apply Lt.lt_n_S
-               | _ => apply Le.le_n_S
-               | _ => apply filter_list_dec
-               | [ H : _ -> _ -> ?G |- ?G ] => apply H; auto
-             end. }
-  Defined.
-  Lemma rdp_list_ntl_wf : forall str, well_founded (@rdp_list_productions_listT_R str).
-  Proof.
-    unfold rdp_list_productions_listT_R.
-    intro.
-    apply well_founded_ltof.
-  Defined.
-End recursive_descent_parser_list.
-
-(*
-
-  Section parse_tree.
-    Context (make_splits : forall (str : String) (pat : production CharType),
-                             list
-                               {str' : String |
-                                Length String str' <= Length _ str}).
-    Local Hint Constructors parse_of parse_of_production parse_of_item : parse_tree.
-    Local Hint Resolve ParseHead ParseProductionSingleton : parse_tree.
-    Local Hint Extern 1 => apply ParseHead : parse_tree.
-    Local Hint Extern 0 (option (parse_of _ _ _ [])) => exact None : parse_tree.
-
-    Definition parse_tree_for : forall str nt, option (parse_of String G str nt).
-    Proof with auto with parse_tree nocore.
-      apply (@parse_productions (fun str nt => option (parse_of _ G str nt))).
-      { intros str name [p|]; [ apply Some | exact None ]... }
-      { intros.
-        specialize (make_splits str).
-        pose proof (fun pat => map (fun spf => exist (fun s => Length _ s <= max_len)
-                                                     (proj1_sig spf)
-                                                     (transitivity (R := le) (proj2_sig spf) pf))
-                                   (make_splits pat)) as make_splits'.
-        specialize (fun pat => parse_production_from_split_list' (make_splits' pat) pat).
-Goal (fun x : nat => x) = (fun x : nat => x).
-  match goal with
-    | |- context[fun x => x] => pose (fun y : Set => y)
-  end. (* success *)
-  match goal with
-    | |- context[fun y => y] => pose (fun y : Set => y)
-  end. (* Toplevel input, characters 0-78:
-Error: Ltac variable y is not bound to an identifier.
-It cannot be used in a binder. *)
-        Variable pick_splits : forall (str : String) (pat : production CharType),
-                                 { strs : list { str' : String | Length _ str' <= Length _ str }
-                                 | fold_left (fun sp acc => proj1_sig (fst sp) ++ acc) (Empty _) (combine strs pat) = str
-                                   /\
-        admit. }
-      { (** decide_leaf *)
-        intros str ch.
-        case_eq (str =s [[ch]]); intro H; [ apply bool_eq_correct in H; apply Some | exact None ].
-        subst... }
-      { (** fold_productions *)
-        intros str pats parses; induction parses; simpl in *...
-        repeat match goal with H : option _ |- _ => destruct H end;
-          try solve [ apply Some; auto with parse_tree nocore
-                    | apply Some;
-                      repeat match goal with
-                               | _ => progress auto with parse_tree nocore
-                               | [ H : parse_of _ _ _ _ |- _ ] => inversion H; clear H; subst
-                             end
-                    | match goal with
-                        | [ H : parse_of _ _ _ _ |- _ ] => fail 1
-                        | _ => idtac
-                      end;
-                      exact None ]. }
-      { (** make_abort *)
-        intros; exact None. }
-    Defined.
-        {
-        apply Some.
-        apply ParseHead.
-        inversion p; subst.
-        try solve [ apply Some.. ].
-
-        auto with parse_tree nocore.
-        .
-
-        exact (fun str ch =>
-                 if str =s [ [ ch ] ] as b return (
-
-Print Universes.
-        apply ParseProductionSingleton.
-        constructor.
-        assumption.
-        eapply ParseProductionCons.
-        Print parse_of_production.
-      Print parse_of.
-
-End recursive_descent_parser.
-
-Section
-*)
-
-
-Section example_parse_string_grammar.
-  Fixpoint make_all_single_splits (str : string) : list { strs : string * string | (fst strs ++ snd strs = str)%string }.
-  Proof.
-    refine ((exist _ (""%string, str) eq_refl)::_).
-    refine (match str with
-              | ""%string => nil
-              | String.String ch str' => map (fun p => exist _ (String.String ch (fst (proj1_sig p)),
-                                                                snd (proj1_sig p))
-                                                             _)
-                                             (make_all_single_splits str')
-            end).
-    simpl; apply f_equal.
-    apply proj2_sig.
-  Defined.
-
-  Lemma length_append (s1 s2 : string) : length (s1 ++ s2) = length s1 + length s2.
-  Proof.
-    revert s2.
-    induction s1; simpl; trivial; [].
-    intros.
-    f_equal; auto.
-  Qed.
-
-  Fixpoint flatten1 {T} (ls : list (list T)) : list T
-    := match ls with
-         | nil => nil
-         | x::xs => (x ++ flatten1 xs)%list
-       end.
-
-  Lemma flatten1_length_ne_0 {T} (ls : list (list T)) (H0 : Datatypes.length ls <> 0)
-        (H1 : Datatypes.length (hd nil ls) <> 0)
-  : Datatypes.length (flatten1 ls) <> 0.
-  Proof.
-    destruct ls as [| [|] ]; simpl in *; auto.
-  Qed.
-
-  Local Ltac t' :=
-    match goal with
-      | _ => progress simpl in *
-      | _ => progress subst
-      | [ H : ?a = ?b |- _ ] => progress subst a
-      | [ H : ?a = ?b |- _ ] => progress subst b
-      | _ => rewrite (LeftId string_stringlike _)
-      | _ => rewrite (RightId string_stringlike _)
-      | _ => reflexivity
-      | _ => split
-      | _ => right; reflexivity
-      | _ => rewrite map_length
-      | _ => rewrite map_map
-      | _ => rewrite length_append
-      | _ => progress destruct_head_hnf prod
-      | _ => progress destruct_head_hnf and
-      | _ => progress destruct_head_hnf or
-      | _ => progress destruct_head_hnf sig
-      | _ => progress auto with arith
-      | _ => apply f_equal
-      | _ => solve [ apply proj2_sig ]
-      | _ => solve [ left; auto with arith ]
-      | [ str : string |- _ ] => solve [ destruct str; simpl; auto with arith ]
-      | [ str : string |- _ ] => solve [ left; destruct str; simpl; auto with arith ]
-    end.
-  Local Ltac t'' :=
-    match goal with
-      | _ => progress t'
-      | [ str : string |- _ ] => solve [ destruct str; repeat t' ]
-    end.
-  Local Ltac t :=
-    solve [ repeat t'' ].
-
-  Local Hint Resolve NPeano.Nat.lt_lt_add_l NPeano.Nat.lt_lt_add_r NPeano.Nat.lt_add_pos_r NPeano.Nat.lt_add_pos_l : arith.
-
-  Definition brute_force_splitter
-  : forall (str : string_stringlike) (pat : production Ascii.ascii),
-      Datatypes.length pat > 0 ->
-      {ls
-       : list
-           {split
-            : list
-                {str_part : string_stringlike | str_part ≤s str } |
-            Datatypes.length split = Datatypes.length pat /\
-            fold_right Concat (Empty string_stringlike)
-                       (map (@proj1_sig _ _) split) = str} |
-       Datatypes.length ls <> 0}.
-  Proof.
-    simpl; unfold str_le in *.
-    intros str [|pat pats] H;
-      [ exfalso; clear str; simpl in H; abstract inversion H
-      | clear H ].
-    revert str.
-    induction pats; simpl in *; intros str.
-    { (** We only get one thing in the list *)
-      refine (exist _ ((exist _ ((exist _ str _)::nil) _)::nil) _).
-      simpl; auto with arith. }
-    { pose (make_all_single_splits str) as single_splits.
-      pose proof (map (@proj1_sig _ _) single_splits).
-      pose proof (fun str => map (map (@proj1_sig _ _)) (map (@proj1_sig _ _) (proj1_sig (IHpats str)))).
-      let P := match goal with |- sig ?P => constr:P end in
-      refine (exist
-                P
-                (flatten1
-                   (map (fun s1s2p =>
-                           map
-                             (fun split_list => exist
-                                                  _
-                                                  (((exist _ (fst (proj1_sig s1s2p)) _)
-                                                      ::(map (fun s => exist _ (proj1_sig s) _)
-                                                             (proj1_sig split_list))))
-                                                  _)
-                             (proj1_sig (IHpats (snd (proj1_sig s1s2p)))))
-                        single_splits))
-                _).
-      apply flatten1_length_ne_0; simpl.
-      { rewrite !map_length; subst_body; simpl; clear;
-        abstract (destruct str; simpl; auto with arith). }
-      { subst_body;
-        destruct str; simpl.
-        { rewrite map_length; clear; abstract t. }
-        { rewrite map_length; clear; abstract t. } } }
-    Grab Existential Variables.
-    { simpl. split.
-      { rewrite map_length; clear; abstract t. }
-      { subst_body; rewrite map_map; simpl; abstract t. } }
-    { abstract t. }
-    { abstract t. }
-    { simpl; abstract t. }
-    { abstract t. }
-  Defined.
-
-  Variable G : grammar Ascii.ascii.
-
-  Definition brute_force_make_parse_of : forall str nt, parse_of string_stringlike G str nt
-                                            + option (parse_of string_stringlike G str nt -> False).
-  Proof.
-    eapply parse_tree_for
-    with (productions_listT := rdp_list_productions_listT)
-           (is_valid_productions := rdp_list_is_valid_productions Ascii.ascii_dec)
-           (remove_productions := rdp_list_remove_productions Ascii.ascii_dec)
-           (productions_listT_R := rdp_list_productions_listT_R).
-    { intros; exact (Valid_nonterminals G). }
-    { apply rdp_list_remove_productions_dec. }
-    { apply rdp_list_ntl_wf. }
-    { apply brute_force_splitter. }
-  Defined.
-End example_parse_string_grammar.
-
-Module example_parse_empty_grammar.
-  Definition make_parse_of : forall str nt, parse_of string_stringlike (trivial_grammar _) str nt
-                                            + option (parse_of string_stringlike (trivial_grammar _) str nt -> False)
-    := @brute_force_make_parse_of (trivial_grammar _).
-
-
-
-  Definition parse : forall str : string,
-                       (parse_of string_stringlike (trivial_grammar _) str (trivial_grammar _))
-                       + option ((parse_of string_stringlike (trivial_grammar _) str (trivial_grammar _)) -> False)
-    := fun str => make_parse_of str _.
-
-  Eval hnf in if (parse "") then true else false.
-  Eval hnf in if (parse "a") then true else false.
-
-  Arguments eq_rect_r / .
-  Arguments eq_rec_r / .
-  Arguments eq_ind_r / .
-
-  Goal True.
-    pose (parse "") as X.
-    hnf in X; simpl in X.
-    pose (parse "a") as Y.
-    hnf in Y; simpl in Y.
-  Abort.
-End example_parse_empty_grammar.
-
-
-Section examples.
-  Section ab_star.
-
-    Fixpoint production_of_string (s : string) : production Ascii.ascii
-      := match s with
-           | EmptyString => nil
-           | String.String ch s' => (Terminal ch)::production_of_string s'
-         end.
-
-    Coercion production_of_string : string >-> production.
-
-    Definition ab_star_grammar : grammar Ascii.ascii :=
-      {| Start_symbol := "ab_star";
-         Lookup := fun s =>
-                     if string_dec s ""
-                     then nil::nil
-                     else if string_dec s "ab"
-                          then ("ab"%string : production _)::nil
-                          else if string_dec s "ab_star"
-                               then ((NonTerminal _ ""%string)::nil)
-                                      ::((NonTerminal _ "ab"%string)::(NonTerminal _ "ab_star")::nil)
-                                      ::nil
-                               else nil::nil;
-         Valid_nonterminal_symbols := (""::"ab"::"ab_star"::nil)%string |}.
-
-    Definition make_parse_of : forall (str : string)
-                                      (prods : productions Ascii.ascii),
-                                 _
-      := @brute_force_make_parse_of ab_star_grammar.
-
-
-
-    Definition parse : forall str : string, _
-      := fun str => make_parse_of str ab_star_grammar.
-(*
-    Time Eval hnf in if parse "" then true else false.
-    Check eq_refl : parse "" = true.
-    Time Compute parse "a".
-    Check eq_refl : parse "a" = false.
-    Time Compute parse "ab".
-    Check eq_refl : parse "ab" = true.
-    Time Compute parse "aa".
-    Check eq_refl : parse "aa" = false.
-    Time Compute parse "ba".
-    Check eq_refl : parse "ba" = false.
-    Time Compute parse "aba".
-    Check eq_refl : parse "aba" = false.
-    Time Compute parse "abab".
-    Check eq_refl : parse "abab" = true.*)
-  (* For debugging: *)(*
-  Goal True.
-    pose proof (eq_refl (parse "abab")) as s.
-    unfold parse in s.
-    unfold make_parse_of in s.
-    unfold brute_force_make_parse_of in s.
-    cbv beta zeta delta [parse_productions] in s.
-    cbv beta zeta delta [parse_productions_or_abort] in s.
-    rewrite Init.Wf.Fix_eq in s.
-    Ltac do_compute_in c H :=
-      let c' := (eval compute in c) in
-      change c with c' in H.
-    do_compute_in (lt_dec (Length string_stringlike "abab"%string) (Length string_stringlike "abab"%string)) s.
-    change (if in_right then ?x else ?y) with y in s.
-    cbv beta zeta delta [rdp_list_is_valid_productions] in s.
-                       *)
-  End ab_star.
-End examples.
